QR_ZK.ec
@@ -1,0 +1,101 @@
+require import AllCore List.
+require import QR_Basics.
+
+
+require Iterated_Failure.
+clone import Iterated_Failure as IF with type irt <- (qr_c * qr_w),
+                                         type rrt <- bool * bool list,
+                                         type sbits <- sbits.
+
+
+
+require Mywhile.
+clone import Mywhile as MW with type irt <- (qr_c * qr_w),
+                                         type rrt <- bool * bool list.
+
+
+require RewBasics.
+clone import RewBasics as RW with type sbits <- sbits,
+                                  type iat   <- iat,
+                                  type iat2  <- (qr_c * qr_w),
+                                  type rrt   <- bool * bool list,
+                                  type irt   <- (qr_c * qr_w),
+                                  op pair_sbits <- pair_sbits,
+                                  op unpair <- unpair.
+                                         
+
+module type RewVerifierA = {
+  proc challenge(Ny : qr_c, c : int) : bool 
+  proc summitup(c : int, b : bool, r : int) : bool list 
+  proc getState() : sbits
+  proc * setState(b : sbits) : unit 
+}.
+
+
+module A(V : RewVerifierA) = {
+  module S = Sim1(V)
+  proc getState() : sbits = {
+    return witness;
+  }
+  proc setState(s : sbits) = {
+    V.setState(s);
+    Sim1.result <- witness;
+  }
+
+  proc run(i : qr_c * qr_w) : bool * bool list = {
+    var r; 
+    r <- S.simulate(fst i);
+    return r;
+  }
+
+}.
+
+
+
+section.
+declare module V : RewVerifierA {HP,WW,W}.
+
+
+
+
+axiom A_ll : islossless GetRunSet(A(V)).main.
+axiom A_ll2 :   islossless A(V).run.
+local lemma qrp_zk2_pr (e ja : int) q &m Na ya (wa : qr_w) : 
+    0 <= ja - 2 =>
+  ja <= e + 1 =>
+    IsSqRoot (Na, ya) wa =>
+    Pr[ W(A(V)).whp_A(fst, ((Na,ya),wa), 1,e,(false,[])) @ &m :
+       W.c = ja /\ (fst res) /\ q (snd res) ]
+        = (1%r/2%r)^(ja - 2) * ((1%r/2%r) * Pr[ZK(HP, V).main(Na,ya,wa) @ &m : q res ]).
+move => jap1 jap2 isr.
+
+have <-: Pr[ WW(GetRunSet(A(V))).whp(fst,((Na,ya),wa),1,e,(false,[])) @ &m : WW.c = ja /\ fst res /\ q (snd res) ]  
+  = Pr[W(A(V)).whp_A(fst, ((Na, ya), wa), 1, e,
+      (false, [])) @ &m : W.c = ja /\ res.`1 /\ q res.`2].
+byequiv (_: ={glob A, glob V,arg} ==> WW.c{1} = W.c{2} /\ ={res}).
+proc. sp.  sim. auto. auto.
+
+apply (whp_cap_fin (GetRunSet(A(V))) A_ll &m fst (fun x => q (snd x)) ((Na,ya),wa) e (false,[]) ja (1%r / 2%r * Pr[ZK(HP, V).main(Na, ya, wa) @ &m : q res]) (fun x => (1%r/2%r)^x)  )  .
+auto. auto. auto. simplify.
+
+bypr. progress.   admit.
+
+progress. bypr.
+move => &n. elim.  move => ap ge. rewrite ap. simplify.
+have ->: Pr[WW(GetRunSet(A(V))).whp(fst, ((Na,ya),wa), 1, ea, (false,[])) @ &n : ! fst res]
+ = Pr[W(A(V)).whp_A(fst, ((Na,ya),wa), 1, ea, (false,[])) @ &m : ! fst res].
+byequiv (_: ={glob A, glob V,arg} ==> ={res}).
+proc. sp. sim. auto. 
+auto.
+
+apply (final_zz (A(V)) A_ll2 _ &m) .
+admit. 
+auto. auto. simplify. 
+byphoare. 
+proc.
+
+call (simnres V).
+admit.
+skip. auto. auto. auto. 
+admit.
+qed.
